wip the main correctness proof of the processor impl.

Kami/Ex/PipelinedProc.v
@@ -20,28 +20,32 @@ Section PipelinedProc.
                "val" :: dataK
              }.
     
-    Definition regFile := MODULE {
-      Register "rf" : Vector dataK rfSize <- rfInit
-
-      with Method "rfRead1" (idx: Bit rfSize): dataK :=
-        Read rf <- "rf";
-        Ret #rf@[#idx]
-
-      with Method "rfRead2" (idx: Bit rfSize): dataK :=
-        Read rf <- "rf";
-        Ret #rf@[#idx]
-
-      with Method "rfWrite" (wr: Struct RfWrite): Void :=
-        Read rf <- "rf";
-        Write "rf" <- #rf@[#wr!RfWrite@."idx" <- #wr!RfWrite@."val"];
-        Retv
-    }.
-      
+    Definition regFile :=
+      MODULE {
+        Register "rf" : Vector dataK rfSize <- rfInit
+        with Method "rfRead1" (idx: Bit rfSize): dataK :=
+          Read rf <- "rf";
+          Ret #rf@[#idx]
+        with Method "rfRead2" (idx: Bit rfSize): dataK :=
+          Read rf <- "rf";
+          Ret #rf@[#idx]
+        with Method "rfWrite" (wr: Struct RfWrite): Void :=
+          Read rf <- "rf";
+          Write "rf" <- #rf@[#wr!RfWrite@."idx" <- #wr!RfWrite@."val"];
+          Retv
+      }.
+    Lemma regFile_PhoasWf: ModPhoasWf regFile.
+    Proof. kequiv. Qed.
+    Lemma regFile_RegsWf: ModRegsWf regFile.
+    Proof. kvr. Qed.
+    
     Definition rfRead1 := MethodSig "rfRead1"(Bit rfSize): dataK.
     Definition rfRead2 := MethodSig "rfRead2"(Bit rfSize): dataK.
     Definition rfWrite := MethodSig "rfWrite"(Struct RfWrite): Void.
 
   End RegFile.
+
+  Hint Resolve regFile_PhoasWf regFile_RegsWf.
 
   Definition D2E :=
     STRUCT { "op" :: opK;
@@ -81,9 +85,15 @@ Section PipelinedProc.
           Write "pc" <- #pc + $1;
           Retv
         }.
+    Lemma decoder_PhoasWf: ModPhoasWf decoder.
+    Proof. kequiv. Qed.
+    Lemma decoder_RegsWf: ModRegsWf decoder.
+    Proof. kvr. Qed.
 
   End Decoder.
-    
+
+  Hint Resolve decoder_PhoasWf decoder_RegsWf.
+  
   Definition scoreboard :=
     MODULE {
       Register "sbFlags" : Vector Bool rfSize <- Default
@@ -110,7 +120,13 @@ Section PipelinedProc.
         Write "sbFlags" <- #flags@[#nidx <- $$false];
         Retv
     }.
+  Lemma scoreboard_PhoasWf: ModPhoasWf scoreboard.
+  Proof. kequiv. Qed.
+  Lemma scoreboard_RegsWf: ModRegsWf scoreboard.
+  Proof. kvr. Qed.
 
+  Hint Resolve scoreboard_PhoasWf scoreboard_RegsWf.
+  
   Definition sbSearch1 := MethodSig "sbSearch1"(Bit rfSize) : Bool.
   Definition sbSearch2 := MethodSig "sbSearch2"(Bit rfSize) : Bool.
   Definition sbSearch3 := MethodSig "sbSearch3"(Bit rfSize) : Bool.
@@ -195,30 +211,61 @@ Section PipelinedProc.
           Call toHost(#val1);
           Retv
       }.
-
+    Lemma executer_PhoasWf: ModPhoasWf executer.
+    Proof. kequiv. Qed.
+    Lemma executer_RegsWf: ModRegsWf executer.
+    Proof. kvr. Qed.
+    
   End Executer.
 
+  Hint Resolve executer_PhoasWf executer_RegsWf.
+  
   Definition writeback :=
     MODULE {
       Rule "writeback" :=
         Call e2w <- e2wDeq();
         Call rfWrite(#e2w);
+        Call sbRemove(#e2w!RfWrite@."idx");
         Retv
     }.
+  Lemma writeback_PhoasWf: ModPhoasWf writeback.
+  Proof. kequiv. Qed.
+  Lemma writeback_RegsWf: ModRegsWf writeback.
+  Proof. kvr. Qed.
+  Hint Resolve writeback_PhoasWf writeback_RegsWf.
 
-  Definition procImpl (init: ProcInit instK dataK rfSize pgmSize) :=
-    ((regFile (rfInit init))
-       ++ (decoder (pcInit init) (pgmInit init))
-       ++ d2e
-       ++ executer
+  Variable (init: ProcInit instK dataK rfSize pgmSize).
+  
+  Definition procImpl :=
+    (((decoder (pcInit init) (pgmInit init))
+        ++ d2e
+        ++ executer)
+       ++ (regFile (rfInit init))
        ++ e2w
        ++ scoreboard
        ++ writeback)%kami.
-
-  Definition procMemImpl (init: ProcInit instK dataK rfSize pgmSize) :=
-    (procImpl init ++ memory dataK addrSize)%kami.
+  Lemma procImpl_PhoasWf: ModPhoasWf procImpl.
+  Proof. kequiv. Qed.
+  Lemma procImpl_RegsWf: ModRegsWf procImpl.
+  Proof. kvr. Qed.
+  Hint Resolve procImpl_PhoasWf procImpl_RegsWf.
+  
+  Definition procMemImpl :=
+    (procImpl ++ memory dataK addrSize)%kami.
+  Lemma procMemImpl_PhoasWf: ModPhoasWf procMemImpl.
+  Proof. kequiv. Qed.
+  Lemma procMemImpl_RegsWf: ModRegsWf procMemImpl.
+  Proof. kvr. Qed.
 
 End PipelinedProc.
+
+Hint Resolve regFile_PhoasWf regFile_RegsWf.
+Hint Resolve decoder_PhoasWf decoder_RegsWf.
+Hint Resolve scoreboard_PhoasWf scoreboard_RegsWf.
+Hint Resolve executer_PhoasWf executer_RegsWf.
+Hint Resolve writeback_PhoasWf writeback_RegsWf.
+Hint Resolve procImpl_PhoasWf procImpl_RegsWf.
+Hint Resolve procMemImpl_PhoasWf procMemImpl_RegsWf.
 
 Hint Unfold regFile d2e decoder scoreboard e2w executer writeback
      procImpl procMemImpl: ModuleDefs.
