Kami/Ex/ProcMemOk.v
@@ -1,50 +1,170 @@
 Require Import Kami.
-Require Import Lib.Indexer.
-Require Import Ex.Fifo Ex.PipelinedProc Ex.DecExec.
+Require Import Lib.FinNotations Lib.Struct Lib.Indexer.
+Require Import Ex.OneEltFifo Ex.ProcMemSpec Ex.PipelinedProc Ex.DecExec.
 
-Require Import Kami.Tactics.
+Require Import Kami.Tactics Kami.ModuleBoundEx.
 
-(* Lemma procMemImpl_ModEquiv: *)
-(*   forall (instK dataK: Kind) (addrSize rfSize pgmSize fifoSize: nat) *)
-(*          (dec: Decoder instK addrSize rfSize) *)
-(*          (exec: Executer dataK) *)
-(*          (init: ProcInit instK dataK addrSize rfSize pgmSize), *)
-(*     ModEquiv type typeUT (procMemImpl fifoSize dec exec init). *)
-(* Proof. *)
-(*   kequiv. *)
-(* Qed. *)
-(* Hint Resolve procMemImpl_ModEquiv. *)
+Section PipelinedProc.
+  Variables (instK dataK: Kind)
+            (addrSize rfSize: nat)
+            (pgmSize: nat).
 
-(* Definition procMemInl *)
-(*            (instK dataK: Kind) (addrSize rfSize pgmSize fifoSize: nat) *)
-(*            (dec: Decoder instK addrSize rfSize) *)
-(*            (exec: Executer dataK) *)
-(*            (init: ProcInit instK dataK addrSize rfSize pgmSize) *)
-(*   : sigT (fun m: Modules => (procMemImpl fifoSize dec exec init) <<== m). *)
-(* Proof. *)
-(*   pose proof (inlineF_refines *)
-(*                 (procMemImpl_ModEquiv fifoSize dec exec init) *)
-(*                 (Reflection.noDupStr_NoDup *)
-(*                    (Struct.namesOf *)
-(*                       (getDefsBodies *)
-(*                          (procMemImpl fifoSize dec exec init))) *)
-(*                    eq_refl)) as Him. *)
-(*   unfold MethsT in Him; rewrite <-SemFacts.idElementwiseId in Him. *)
-(*   match goal with *)
-(*   | [H: context[inlineF ?m] |- _] => set m as origm in H at 2 *)
-(*   end. *)
-(*   kinline_compute_in Him. *)
-(*   unfold origm in *. *)
-(*   specialize (Him eq_refl). *)
-(*   exact (existT _ _ Him). *)
-(* Defined. *)
+  Variables (dec: Decoder instK addrSize rfSize)
+            (exec: Executer dataK).
 
-(* Theorem procMemImpl_ok: *)
-(*   forall (instK dataK: Kind) (addrSize rfSize pgmSize fifoSize: nat) *)
-(*          (dec: Decoder instK addrSize rfSize) *)
-(*          (exec: Executer dataK) *)
-(*          (init: ProcInit instK dataK addrSize rfSize pgmSize), *)
-(*     procMemImpl fifoSize dec exec init <<== procMemSpec dec exec init. *)
-(* Proof. *)
-(* Admitted. *)
+  Variable (init: ProcInit instK dataK rfSize pgmSize).
+  
+  Definition procImpl2 :=
+    ((decexec dec exec (pcInit init) (pgmInit init))
+       ++ (regFile (rfInit init))
+       ++ (e2w dataK rfSize)
+       ++ (scoreboard rfSize)
+       ++ (writeback dataK rfSize))%kami.
+  Lemma procImpl2_PhoasWf: ModPhoasWf procImpl2.
+  Proof. kequiv. Qed.
+  Lemma procImpl2_RegsWf: ModRegsWf procImpl2.
+  Proof. kvr. Qed.
+  Hint Resolve procImpl2_PhoasWf procImpl2_RegsWf.
+
+  Hint Unfold procImpl2: ModuleDefs.
+  
+  Theorem procImpl2_ok:
+    procImpl dec exec init <<== procImpl2.
+  Proof.
+    kmodular.
+    - apply decexec_ok.
+    - krefl.
+  Qed.
+
+  (* Eval vm_compute in (namesOf (getRegInits procImpl2)). *)
+  (* = ["pc"%string; "pgm"%string; "rf"%string; "elt.e2w"%string; *)
+  (*    "full.e2w"%string; "sbFlags"%string] *)
+  (*   : list string *)
+  (* Eval vm_compute in (namesOf (getRegInits (procSpec dec exec init))). *)
+  (* = ["pc"%string; "rf"%string; "pgm"%string] *)
+  (*   : list string *)
+  (** FIXME *)
+  Definition procImpl2_regMap (r: RegsT): RegsT :=
+    (mlet pcv: (Bit pgmSize) <- r |> "pc";
+       mlet pgmv: (Vector instK pgmSize) <- r |> "pgm";
+       mlet rfv: (Vector dataK rfSize) <- r |> "rf";
+       mlet e2wfullv: Bool <- r |> "e2w"--"full";
+       mlet e2weltv: (Struct (RfWrite dataK rfSize)) <- r |> "e2w"--"elt";
+       mlet sbFlagsv: (Vector Bool rfSize) <- r |> "sbFlags";
+       (["pgm" <- existT _ _ pgmv]
+        +["rf" <- existT _ _ rfv]
+        +["pc" <- existT _ _ pcv])%fmap)%mapping.
+  Hint Unfold procImpl2_regMap: MapDefs.
+
+  (* Eval vm_compute in (namesOf (getRules procImpl2)). *)
+  (* = ["decexecArith"%string; "decexecLd"%string; *)
+  (*    "decexecSt"%string; "decexecTh"%string; *)
+  (*    "writeback"%string] *)
+  (*   : list string *)
+  (* Eval vm_compute in (namesOf (getRules (procSpec dec exec init))). *)
+  (* = ["doArith"%string; "doLoad"%string; "doStore"%string; *)
+  (*    "doToHost"%string] *)
+  (*   : list string *)
+  Definition procImpl2_ruleMap (o: RegsT): string -> option string :=
+    "decexecArith" |-> "doArith";
+      "decexecLd" |-> "doLoad";
+      "decexecSt" |-> "doStore";
+      "decexecTh" |-> "doToHost"; ||.
+  Hint Unfold procImpl2_ruleMap: MethDefs.
+
+  Definition procImpl2Inl: sigT (fun m: Modules => procImpl2 <<== m).
+  Proof.
+    pose proof (inlineF_refines
+                  (procImpl2_PhoasWf type typeUT)
+                  (Reflection.noDupStr_NoDup
+                     (namesOf (getDefsBodies procImpl2))
+                     eq_refl)) as Him.
+    unfold MethsT in Him; rewrite <-SemFacts.idElementwiseId in Him.
+    match goal with
+    | [H: context[inlineF ?m] |- _] => set m as origm in H at 2
+    end.
+    kinline_compute_in Him.
+    unfold origm in *.
+    specialize (Him eq_refl).
+    exact (existT _ _ Him).
+  Defined.
+
+  (* Eval vm_compute in (namesOf (getRegInits procImpl2)). *)
+  (* = ["pc"%string; "pgm"%string; "rf"%string; "elt.e2w"%string; *)
+  (*    "full.e2w"%string; "sbFlags"%string] *)
+  (*   : list string *)
+  Record procImpl2_inv (o: RegsT): Prop :=
+    { pcv: fullType type (SyntaxKind (Bit pgmSize));
+      Hpcv: M.find "pc"%string o = Some (existT _ _ pcv);
+      pgmv: fullType type (SyntaxKind (Vector instK pgmSize));
+      Hpgmv: M.find "pgm"%string o = Some (existT _ _ pgmv);
+      e2wfullv: fullType type (SyntaxKind Bool);
+      He2wfullv: M.find "full.e2w"%string o = Some (existT _ _ e2wfullv);
+      e2weltv: fullType type (SyntaxKind (Struct (RfWrite dataK rfSize)));
+      He2weltv: M.find "elt.e2w"%string o = Some (existT _ _ e2weltv);
+      sbFlagsv: fullType type (SyntaxKind (Vector Bool rfSize));
+      HsbFlagsv: M.find "sbFlags"%string o = Some (existT _ _ sbFlagsv)
+    }.
+  (* Hint Unfold procImpl2_inv_body : InvDefs. *)
+
+  Ltac procImpl2_inv_tac :=
+    try match goal with
+        | [H: procImpl2_inv _ |- _] => destruct H
+        end;
+    kinv_red;
+    econstructor; (* let's prove that the invariant holds for the next state *)
+    try (findReify; (reflexivity || eassumption); fail);
+    kinv_red; (* unfolding invariant definitions *)
+    repeat (* cheaper than "intuition" *)
+      (match goal with
+       | [ |- _ /\ _ ] => split
+       end);
+    try eassumption; intros; try reflexivity;
+    intuition kinv_simpl; intuition idtac.
+
+  Lemma procImpl2_inv_ok':
+    forall init n ll,
+      init = initRegs (getRegInits (projT1 procImpl2Inl)) ->
+      Multistep (projT1 procImpl2Inl) init n ll ->
+      procImpl2_inv n.
+  Proof.
+    induction 2.
+    - unfold getRegInits, procImpl2Inl, projT1.
+      procImpl2_inv_tac; simpl in *; kinv_simpl.
+    - kinvert.
+      + mred.
+      + mred.
+      + kinv_dest_custom procImpl2_inv_tac.
+      + kinv_dest_custom procImpl2_inv_tac.
+      + kinv_dest_custom procImpl2_inv_tac.
+      + kinv_dest_custom procImpl2_inv_tac.
+      + kinv_dest_custom procImpl2_inv_tac.
+  Qed.
+
+  Lemma procImpl2_inv_ok:
+    forall o,
+      reachable o (projT1 procImpl2Inl) ->
+      procImpl2_inv o.
+  Proof.
+    intros; inv H; inv H0.
+    eapply procImpl2_inv_ok'; eauto.
+  Qed.
+
+  Theorem procImpl_ok: procImpl2 <<== procSpec dec exec init.
+  Proof.
+    intros.
+
+    (* 1) inlining *)
+    ketrans; [exact (projT2 procImpl2Inl)|].
+
+    (* 2) decomposition *)
+    kdecompose_nodefs procImpl2_regMap procImpl2_ruleMap.
+
+    (* (* 3) simulation *) *)
+    kinv_add procImpl2_inv_ok.
+    kinv_add_end.
+    kinvert.
+  Admitted.
+  
+End PipelinedProc.
 
